Test.lean
@@ -1,41 +1,370 @@
 import UpdateDeprecations.Basic
 
-open UpdateDeprecations
+open Lean UpdateDeprecations
 
+/-- info: ([a, b, c], ([], [])) -/
+#guard_msgs in
 run_cmd
-  let fn := "True.hish"
-  let s1 := ".hish and more text"
-  let s2 := "hish and more text"
-  let _s3 := "ish and more text"
-  if findNamespaceMatch fn s1 != some ".hish" then Lean.logInfo "error"
-  if findNamespaceMatch fn s2 != some "hish"  then Lean.logInfo "error"
-  --if findNamespaceMatch fn _s3 != none         then Lean.logInfo "error"
+  let left := "a.b.c".splitOn "."
+  let right := "a.b.c".splitOn "."
+  logInfo m!"{List.getCommon left right}"
 
-/-- info: true -/
+/-- info: ([a, b], ([c], [b', d])) -/
 #guard_msgs in
-#eval
-  let str := "  refine' ⟨_, _⟩"
-  replaceCheck str "_" "?_" 11 == "  refine' ⟨?_, _⟩"
+run_cmd
+  let left := "a.b.c".splitOn "."
+  let right := "a.b.b'.d".splitOn "."
+  logInfo m!"{List.getCommon left right}"
 
-/-- info: true -/
+/-- info: some ((A'.B' h).C) -/
 #guard_msgs in
-#eval
-  let str := "  refine' ⟨_, _⟩"
-  replaceCheck str "" "?" 11 == "  refine' ⟨?_, _⟩"
+run_cmd
+  let recombined := recombineNamespace "A.B.C" "h.C" "A'.B'"
+  logInfo m!"{recombined}"
 
-/-- info: true -/
+/--
+info: some (ok1)
+---
+info: some (True.ok2)
+---
+info: some (True.intro.ok2)
+-/
 #guard_msgs in
-#eval
-  let str := "  refine' ⟨_, _⟩"
-  replaceCheck str "refine'" "refine" 2 == "  refine ⟨_, _⟩"
+run_cmd
+  logInfo m!"{recombineNamespace "hello1" "hello1" "ok1"}"
+  logInfo m!"{recombineNamespace "True.hello2" "hello2" "True.ok2"}"
+  logInfo m!"{recombineNamespace "True.hello2" "True.intro.hello2" "True.ok2"}"
 
-/-- info: true -/
+/- `s.splitOn t` is never `[]`
+#eval
+  let s := ["", "a", "b"]
+  let t := ["", "a", "b"]
+  Id.run do
+  let mut tot := #[]
+  for a in s do
+    for b in t do
+      tot := tot.push <| a.splitOn b
+  return tot.all (· ≠ [])
+-/
+
+/-- info: some ((by exact True.intro : ).hello2) -/
 #guard_msgs in
-#eval
-  let str := "  refine' ⟨_, _⟩"
-  replaceCheck str "'" "" 8 == "  refine ⟨_, _⟩"
+run_cmd Lean.Elab.Command.liftTermElabM do
+  let s := "(by exact True.intro : ).hello2"
+  let fullName := "True.hello2"
+  logInfo m!"{findFirstEnd fullName s}"
 
-open Lean Elab Command
-run_cmd liftTermElabM do
+/-- info: some ((by exact True.intro : ).hello2) -/
+#guard_msgs in
+run_cmd Lean.Elab.Command.liftTermElabM do
+  let s := "(by exact True.intro : ).hello2 and then .hello2. more wi"
+  let fullName := "True.hello2"
+  logInfo m!"{findFirstEnd fullName s}"
+
+set_option linter.deprecated false in
+/--
+info: true
+---
+info: true
+-/
+#guard_msgs in
+run_cmd
+  let msgs1 := (← get).messages.msgs
+  let msgs := (← get).messages.unreported
+  let msgs1WithArray := (← get).messages.msgs.toArray
+  let msgsWithArray := (← get).messages.unreported.toArray
+  logInfo m!"{(← msgs1.mapM (·.toString)).toArray == (← msgs.mapM (·.toString)).toArray}"
+  logInfo m!"{(← msgs1WithArray.mapM (·.toString)) == (← msgsWithArray.mapM (·.toString))}"
+
+/--
+info: some ((← get).messages.unreported)
+---
+info: some ((← get).messages.unreported.toArray)
+-/
+#guard_msgs in
+run_cmd
+  let msgs := "Lean.MessageLog.msgs"
+  let unrep := "Lean.MessageLog.unreported"
+  let recombined := recombineNamespace msgs "(← get).messages.msgs" unrep
+  logInfo m!"{recombined}"
+  let msgsToArray := "(← get).messages.msgs.toArray"
+  let recombined := recombineNamespace msgs msgsToArray unrep
+  logInfo m!"{recombined}"
+
+/-- info: some (hp.More) -/
+#guard_msgs in
+run_cmd
+  logInfo m!"{recombineNamespace "Nat.Prime.ne_two" "hp.ne_two" "Nat.Prime.More"}"
+
+/-- info: some ((Nat.newPrime.More hp).ne_two.symm) -/
+#guard_msgs in
+run_cmd
+  logInfo m!"{recombineNamespace "Nat.Prime.ne_two" "hp.ne_two.symm" "Nat.newPrime.More"}"
+
+/-- info: some ((Nat.newPrime.More hp).ne_two) -/
+#guard_msgs in
+run_cmd
+  logInfo m!"{recombineNamespace "Nat.Prime.ne_two" "hp.ne_two" "Nat.newPrime.More"}"
+
+/-- info: ([a, b, c], ([], ([], []))) -/
+#guard_msgs in
+run_cmd
+  let fullName := "a.b.c"
+  let dotNot := "a.b.c"
+  logInfo m!"{splitWithNamespace fullName dotNot}"
+
+/-- info: ([], ([a, b, c], ([], [a, b, c']))) -/
+#guard_msgs in
+run_cmd
+  let fullName := "a.b.c"
+  let dotNot := "a.b.c'"
+  logInfo m!"{splitWithNamespace fullName dotNot}"
+
+/-- info: ([a, b, c], ([], ([], [d]))) -/
+#guard_msgs in
+run_cmd
+  let fullName := "a.b.c"
+  let dotNot := "a.b.c.d"
+  logInfo m!"{splitWithNamespace fullName dotNot}"
+
+/-- info: ([b, c], ([a], ([a'], [d]))) -/
+#guard_msgs in
+run_cmd
+  let fullName := "a.b.c"
+  let dotNot := "a'.b.c.d"
+  logInfo m!"{splitWithNamespace fullName dotNot}"
+
+/-- info: ([b, c], ([a], ([a'], [d, e]))) -/
+#guard_msgs in
+run_cmd
+  let fullName := "a.b.c"
+  let dotNot := "a'.b.c.d.e"
+  logInfo m!"{splitWithNamespace fullName dotNot}"
+
+/-- info: ([ne_two], ([Nat, Prime], ([hp], [symm]))) -/
+#guard_msgs in
+run_cmd
+  let fullName := "Nat.Prime.ne_two"
+  let dotNot := "hp.ne_two.symm"
+  logInfo m!"{splitWithNamespace fullName dotNot}"
+
+/-- info: some (myNat.find) -/
+#guard_msgs in
+run_cmd
+  logInfo m!"{recombineNamespace "Nat.find" "Nat.find" "myNat.find"}"
+
+/-- info: some (myNat.find) -/
+#guard_msgs in
+run_cmd
+  logInfo m!"{recombineNamespace "Nat.find" "find" "myNat.find"}"
+
+/-- info: some (nat.findNew) -/
+#guard_msgs in
+run_cmd
+  logInfo m!"{recombineNamespace "Nat.find" "find" "nat.findNew"}"
+
+/-- info: some (Nat.Int.findNew) -/
+#guard_msgs in
+run_cmd
+  logInfo m!"{recombineNamespace "Nat.Int.find" "Int.find" "Nat.Int.findNew"}"
+
+/-- info: some (x.findNew) -/
+#guard_msgs in
+run_cmd
+  logInfo m!"{recombineNamespace "Nat.Int.find" "x.find" "Nat.Int.findNew"}"
+
+/-- info: none -/
+#guard_msgs in
+run_cmd
+  logInfo m!"{recombineNamespace "Nat.Int.find" "x.ind" "Nat.Int.findNew"}"
+
+/-- info: ([a, b, c], ([], [])) -/
+#guard_msgs in
+run_cmd
+  let left := "a.b.c".splitOn "."
+  let right := "a.b.c".splitOn "."
+  logInfo m!"{List.getCommon left right}"
+
+/-- info: ([a, b], ([c], [b', d])) -/
+#guard_msgs in
+run_cmd
+  let left := "a.b.c".splitOn "."
+  let right := "a.b.b'.d".splitOn "."
+  logInfo m!"{List.getCommon left right}"
+
+/-- info: some ((A'.B' h).C) -/
+#guard_msgs in
+run_cmd
+  let recombined := recombineNamespace "A.B.C" "h.C" "A'.B'"
+  logInfo m!"{recombined}"
+
+/--
+info: some (ok1)
+---
+info: some (True.ok2)
+---
+info: some (True.intro.ok2)
+-/
+#guard_msgs in
+run_cmd
+  logInfo m!"{recombineNamespace "hello1" "hello1" "ok1"}"
+  logInfo m!"{recombineNamespace "True.hello2" "hello2" "True.ok2"}"
+  logInfo m!"{recombineNamespace "True.hello2" "True.intro.hello2" "True.ok2"}"
+
+/- `s.splitOn t` is never `[]`
+#eval
+  let s := ["", "a", "b"]
+  let t := ["", "a", "b"]
+  Id.run do
+  let mut tot := #[]
+  for a in s do
+    for b in t do
+      tot := tot.push <| a.splitOn b
+  return tot.all (· ≠ [])
+-/
+
+/-- info: some ((by exact True.intro : ).hello2) -/
+#guard_msgs in
+run_cmd Lean.Elab.Command.liftTermElabM do
+  let s := "(by exact True.intro : ).hello2"
+  let fullName := "True.hello2"
+  logInfo m!"{findFirstEnd fullName s}"
+
+/-- info: some ((by exact True.intro : ).hello2) -/
+#guard_msgs in
+run_cmd Lean.Elab.Command.liftTermElabM do
+  let s := "(by exact True.intro : ).hello2 and then .hello2. more wi"
+  let fullName := "True.hello2"
+  logInfo m!"{findFirstEnd fullName s}"
+
+/-- info: some (some string(by exact True.intro : ).ok2 and then .hello2. more wi) -/
+#guard_msgs in
+run_cmd Lean.Elab.Command.liftTermElabM do
+  let beg := "some string"
+  let s := beg ++ "(by exact True.intro : ).hello2 and then .hello2. more wi"
+  let fullName := "True.hello2"
+  let newName := "True.ok2"
+  logInfo m!"{ReplData.newLine ⟨fullName, newName, 0, beg.length⟩ #[s]}"
+
+set_option linter.deprecated false in
+/--
+info: true
+---
+info: true
+-/
+#guard_msgs in
+run_cmd
+  let msgs1 := (← get).messages.msgs
+  let msgs := (← get).messages.unreported
+  let msgs1WithArray := (← get).messages.msgs.toArray
+  let msgsWithArray := (← get).messages.unreported.toArray
+  logInfo m!"{(← msgs1.mapM (·.toString)).toArray == (← msgs.mapM (·.toString)).toArray}"
+  logInfo m!"{(← msgs1WithArray.mapM (·.toString)) == (← msgsWithArray.mapM (·.toString))}"
+
+/--
+info: some ((← get).messages.unreported)
+---
+info: some ((← get).messages.unreported.toArray)
+-/
+#guard_msgs in
+run_cmd
+  let msgs := "Lean.MessageLog.msgs"
+  let unrep := "Lean.MessageLog.unreported"
+  let recombined := recombineNamespace msgs "(← get).messages.msgs" unrep
+  logInfo m!"{recombined}"
+  let msgsToArray := "(← get).messages.msgs.toArray"
+  let recombined := recombineNamespace msgs msgsToArray unrep
+  logInfo m!"{recombined}"
+
+/-- info: some (hp.More) -/
+#guard_msgs in
+run_cmd
+  logInfo m!"{recombineNamespace "Nat.Prime.ne_two" "hp.ne_two" "Nat.Prime.More"}"
+
+/-- info: some ((Nat.newPrime.More hp).ne_two.symm) -/
+#guard_msgs in
+run_cmd
+  logInfo m!"{recombineNamespace "Nat.Prime.ne_two" "hp.ne_two.symm" "Nat.newPrime.More"}"
+
+/-- info: some ((Nat.newPrime.More hp).ne_two) -/
+#guard_msgs in
+run_cmd
+  logInfo m!"{recombineNamespace "Nat.Prime.ne_two" "hp.ne_two" "Nat.newPrime.More"}"
+
+/-- info: ([a, b, c], ([], ([], []))) -/
+#guard_msgs in
+run_cmd
+  let fullName := "a.b.c"
+  let dotNot := "a.b.c"
+  logInfo m!"{splitWithNamespace fullName dotNot}"
+
+/-- info: ([], ([a, b, c], ([], [a, b, c']))) -/
+#guard_msgs in
+run_cmd
+  let fullName := "a.b.c"
+  let dotNot := "a.b.c'"
+  logInfo m!"{splitWithNamespace fullName dotNot}"
+
+/-- info: ([a, b, c], ([], ([], [d]))) -/
+#guard_msgs in
+run_cmd
+  let fullName := "a.b.c"
+  let dotNot := "a.b.c.d"
+  logInfo m!"{splitWithNamespace fullName dotNot}"
+
+/-- info: ([b, c], ([a], ([a'], [d]))) -/
+#guard_msgs in
+run_cmd
+  let fullName := "a.b.c"
+  let dotNot := "a'.b.c.d"
+  logInfo m!"{splitWithNamespace fullName dotNot}"
+
+/-- info: ([b, c], ([a], ([a'], [d, e]))) -/
+#guard_msgs in
+run_cmd
+  let fullName := "a.b.c"
+  let dotNot := "a'.b.c.d.e"
+  logInfo m!"{splitWithNamespace fullName dotNot}"
+
+/-- info: ([ne_two], ([Nat, Prime], ([hp], [symm]))) -/
+#guard_msgs in
+run_cmd
+  let fullName := "Nat.Prime.ne_two"
+  let dotNot := "hp.ne_two.symm"
+  logInfo m!"{splitWithNamespace fullName dotNot}"
+
+/-- info: some (myNat.find) -/
+#guard_msgs in
+run_cmd
+  logInfo m!"{recombineNamespace "Nat.find" "Nat.find" "myNat.find"}"
+
+/-- info: some (myNat.find) -/
+#guard_msgs in
+run_cmd
+  logInfo m!"{recombineNamespace "Nat.find" "find" "myNat.find"}"
+
+/-- info: some (nat.findNew) -/
+#guard_msgs in
+run_cmd
+  logInfo m!"{recombineNamespace "Nat.find" "find" "nat.findNew"}"
+
+/-- info: some (Nat.Int.findNew) -/
+#guard_msgs in
+run_cmd
+  logInfo m!"{recombineNamespace "Nat.Int.find" "Int.find" "Nat.Int.findNew"}"
+
+/-- info: some (x.findNew) -/
+#guard_msgs in
+run_cmd
+  logInfo m!"{recombineNamespace "Nat.Int.find" "x.find" "Nat.Int.findNew"}"
+
+/-- info: none -/
+#guard_msgs in
+run_cmd
+  logInfo m!"{recombineNamespace "Nat.Int.find" "x.ind" "Nat.Int.findNew"}"
+
+/-- info: MyProject/new.lean -/
+#guard_msgs in
+run_cmd
   let fil ← `(build| ././././$(mkIdent `MyProject)/$(mkIdent `new.lean))
-  guard <| toFile fil == "MyProject/new.lean"
+  logInfo m!"{toFile fil}"
